kernel/parray.mli
@@ -3,6 +3,7 @@ type 'a t
 val length  : 'a t -> Uint63.t
 val get     : 'a t -> Uint63.t -> 'a
 val set     : 'a t -> Uint63.t -> 'a -> 'a t
+val destr_set : 'a t -> Uint63.t -> 'a -> 'a t
 val default : 'a t -> 'a 
 val make    : Uint63.t -> 'a -> 'a t
 val init    : Uint63.t -> (int -> 'a) -> 'a -> 'a t
